libs/Misc_Generic_Lemmas.thy
@@ -21,4 +21,34 @@ next
     done
 qed
 
+
+text \<open>Just an alternative characterization of find, 
+  to increase trust in that it actually finds first occurrence.
+\<close>
+
+definition "is_first_elem_with_prop P xs x \<equiv> 
+  \<exists>xs\<^sub>1 xs\<^sub>2. xs = xs\<^sub>1@x#xs\<^sub>2 \<and> P x \<and> (\<forall>x'\<in>set xs\<^sub>1. \<not>P x')"
+
+lemma is_first_elem_with_prop_propI: "is_first_elem_with_prop P xs x \<Longrightarrow> P x"  
+  unfolding is_first_elem_with_prop_def
+  by auto
+  
+lemma find_finds_first: "List.find P xs = Some x 
+  \<longleftrightarrow> is_first_elem_with_prop P xs x"
+  unfolding is_first_elem_with_prop_def
+  apply (rule iffI)
+  subgoal
+    apply (clarsimp simp: List.find_Some_iff)
+    subgoal for i
+      by (auto 0 3
+        simp: in_set_conv_nth Cons_nth_drop_Suc
+        intro: exI[where x="drop (Suc i) xs"] exI[where x="take i xs"])
+    done    
+  subgoal
+    apply (clarsimp simp: List.find_Some_iff)
+    by (metis add_Suc_right length_Cons length_greater_0_conv less_add_same_cancel1 list.simps(3) nth_append nth_append_length nth_mem)
+  done  
+
+
+
 end
